$\ll$
$$
\begin{align}
\underline{A}_{\text{diff}}(M) &= K \underline{a_{0}} \int _{x_{p}= -a / 2}^ {a / 2} \int _{y_{p}= -b / 2}^{b / 2}1 \times \exp(jk_{0}(\alpha x_{p}+ \beta x_{p})) \, dx_{p}  \, dy _{p} \\
&= K \underline{a_{0}} \left[  \frac{- \exp(jk_{0 }\alpha a / 2)- \exp(jk_{0}\alpha (- a / 2))}{jk_{0}\alpha} \right]\left[  \frac{- \exp(jk_{0 }\beta b / 2)- \exp(jk_{0}\beta (- b / 2))}{jk_{0}\beta} \right] \\
&= K \underline{a_{0}} \frac{a}{2} \frac{b}{2 }\left[  \frac{2j \sin(k_{0}\alpha a/2)}{jk_{0} \alpha a/2} \right]\left[  \frac{2j \sin(k_{0}\beta b/2)}{jk_{0} \beta b/2} \right]  \\
I_{\text{diff}}(M) &= |\underline{A}_{\text{diff}}|^2 \\
&=|K^2\underline{a_{0} }ab|^2\mathrm{sinc}^2\left(  \frac{2\pi}{\lambda_{0} } \alpha \frac{a}{2} \right) \mathrm{sinc}^2\left(  \frac{2\pi }{\lambda_{0}} \beta  \frac{b}{2} \right)
\end{align}
$$
$$
\underline{A}_{\text{diff}}(M) = K \underline{a}_{0}. \frac{2\pi}{(k_{0}\sin \theta)^ 2} [xJ_{1}(x)]_{0}^{k_{0}a \sin \theta} 
$$

$$
I(\theta) = I_{0 }\left( \frac{2J_{1}(k_{0}a \sin \theta)}{k_{0}a \sin \theta} \right)^2
$$
